src/tools/symbexec/bir_symbLib.sig
@@ -3,31 +3,21 @@ sig
 
   include Abbrev;
 
-  val birs_simp_select : (term -> thm) ref;
-
-  val pcond_gen_symb : term;
-
-  val bir_symb_analysis_init_gen : term option -> term -> term -> thm -> term * thm * thm;
-
-  val bir_symb_analysis : term -> term list -> term -> thm;
-
-  val bir_symb_analysis_thm : thm -> thm -> thm list -> thm -> thm -> thm * thm;
-
-  val bir_symb_analysis_thm_gen : term option -> thm -> thm -> thm list -> thm -> thm -> thm * thm;
+  val bir_symb_analysis_thm : thm -> thm -> thm list -> thm -> thm -> thm;
 
   val bir_symb_transfer :
     term -> term ->
     term -> term ->
     thm -> thm ->
     thm -> thm -> thm ->
-    thm -> thm -> thm ->
+    thm -> thm ->
     thm;
 
   val bir_symb_transfer_thm :
     thm -> thm -> thm ->
     thm -> thm ->
     thm -> thm ->
-    thm -> thm -> thm ->
+    thm -> thm ->
     thm;
 
   val bir_symb_transfer_two :
@@ -35,7 +25,7 @@ sig
     term -> term -> term ->
     thm -> thm ->
     thm -> thm -> thm -> thm ->
-    thm -> thm -> thm ->
+    thm -> thm ->
     thm;
 
   val bir_symb_transfer_two_thm :
@@ -43,7 +33,7 @@ sig
     thm -> thm -> thm ->
     thm -> thm -> thm ->
     thm -> thm ->
-    thm -> thm -> thm ->
+    thm -> thm ->
     thm;
 
 end
