src/tools/symbexec/birs_strategiesLib.sml
@@ -1,0 +1,86 @@
+structure birs_strategiesLib =
+struct
+
+local
+
+  open HolKernel Parse boolLib bossLib;
+
+  open birsSyntax;
+  open birs_utilsLib;
+
+  (* error handling *)
+  val libname = "birs_strategiesLib"
+  val ERR = Feedback.mk_HOL_ERR libname
+  val wrap_exn = Feedback.wrap_exn libname
+
+in (* local *)
+
+  fun not_at_lbls stop_lbls st =
+    not (List.exists (identical (dest_birs_state_pc st)) stop_lbls);
+
+  (* TODO: later make the whole post step function a parameter to the symb_analysis function *)
+  val birs_simp_select = ref birs_simp_instancesLib.birs_simp_default_riscv;
+
+  fun birs_post_step_riscv_default (birs_rule_SUBST_thm) =
+    let
+      val timer_symbanalysis = holba_miscLib.timer_start 0;
+      val timer_symbanalysis_last = ref (holba_miscLib.timer_start 0);
+
+      open birs_execLib;
+      fun birs_post_step_fun (t, (last_pc, last_stmt)) = (
+        (fn t => (
+        holba_miscLib.timer_stop (fn delta_s => print ("running since " ^ delta_s ^ "\n")) timer_symbanalysis;
+        holba_miscLib.timer_stop (fn delta_s => print ("time since last step " ^ delta_s ^ "\n")) (!timer_symbanalysis_last);
+        timer_symbanalysis_last := holba_miscLib.timer_start 0;
+        (*print_term ((last o pairSyntax.strip_pair o snd o dest_comb o concl) t);*)
+        t)) o
+        birs_if_assign_RULE last_stmt (birs_rule_SUBST_trysimp_fun birs_rule_SUBST_thm (!birs_simp_select)) o
+        birs_rule_tryprune_fun birs_rulesTheory.branch_prune1_spec_thm o
+        birs_rule_tryprune_fun birs_rulesTheory.branch_prune2_spec_thm o
+        birs_rule_tryjustassert_fun true
+      ) t;
+    in
+      birs_post_step_fun
+    end;
+
+  fun birs_post_step_armcm0_default (birs_rule_SUBST_thm) =
+    let
+      open birs_simp_instancesLib;
+      val birs_simp_select = birs_simp_default_armcm0_gen true;
+      val birs_simp_select_ifthenelse = birs_simp_default_core_exp_simp;
+      open holba_miscLib;
+
+      val timer_symbanalysis = timer_start 0;
+      val timer_symbanalysis_last = ref (timer_start 0);
+      fun debug_output_RULE t =
+         (timer_stop (fn delta_s => print ("running since " ^ delta_s ^ "\n")) timer_symbanalysis;
+         timer_stop (fn delta_s => print ("time since last step " ^ delta_s ^ "\n")) (!timer_symbanalysis_last);
+         timer_symbanalysis_last := timer_start 0;
+         (*print_term ((last o pairSyntax.strip_pair o snd o dest_comb o concl) t);*)
+         t);
+
+      open birs_execLib;
+      val birs_simp_RULE_gen = birs_rule_SUBST_trysimp_fun birs_rule_SUBST_thm;
+      fun birs_simp_RULE last_stmt =
+        ((* the ifthenelse simplification for countw assignments before branches, that gets applied after the branch happens and the condition is available in the branchcondition *)
+         birs_if_branch_RULE (birs_simp_RULE_gen (birs_simp_select_ifthenelse)) o
+         (* the simplification after assignments *)
+         birs_if_assign_RULE last_stmt (birs_simp_RULE_gen (birs_simp_select)));
+      val birs_prune_RULE =
+        (birs_rule_tryprune_fun birs_rulesTheory.branch_prune1_spec_thm o
+         birs_rule_tryprune_fun birs_rulesTheory.branch_prune2_spec_thm o
+         birs_rule_tryjustassert_fun true);
+
+      fun birs_post_step_fun (t, (last_pc, last_stmt)) = (
+         debug_output_RULE o
+         (*(apply_if_branch debug_Pi_fun) o*)
+         birs_simp_RULE last_stmt o
+         birs_prune_RULE
+      ) t;
+    in
+      birs_post_step_fun
+    end;
+
+end (* local *)
+
+end (* struct *)
