examples/riscv/incr-mem/incr_mem_symb_execScript.sml
@@ -13,17 +13,13 @@ val _ = new_theory "incr_mem_symb_exec";
 (* Symbolic analysis execution *)
 (* --------------------------- *)
 
-val (bsysprecond_thm, symb_analysis_thm) =
+val symb_analysis_thm =
  bir_symb_analysis_thm
   bir_incr_mem_prog_def
   incr_mem_init_addr_def [incr_mem_end_addr_def]
   bspec_incr_mem_pre_def incr_mem_birenvtyl_def;
 
 val _ = show_tags := true;
-
-val _ = Portable.pprint Tag.pp_tag (tag bsysprecond_thm);
-
-Theorem incr_mem_bsysprecond_thm = bsysprecond_thm
 
 val _ = Portable.pprint Tag.pp_tag (tag symb_analysis_thm);
 
