src/tools/symbexec/bir_symbLib.sml
@@ -13,77 +13,9 @@ local
   open bitTheory;
   open birs_auxTheory;
   open bir_immSyntax;
-
-  local
-    open bir_programSyntax;
-    open optionSyntax;
-    fun is_SOME_BStmtB_BStmt_Assign t = is_some t andalso (is_BStmtB o dest_some) t andalso (is_BStmt_Assign o dest_BStmtB o dest_some) t;
-  in
-    fun apply_if_assign tm f =
-      if is_SOME_BStmtB_BStmt_Assign tm then
-        f
-      else
-        I;
-  end
 in
 
-(* TODO: later make the whole post step function a parameter to the symb_analysis function *)
-val birs_simp_select = ref birs_simp_instancesLib.birs_simp_default_riscv;
-
-val pcond_gen_symb = ``BVar "syp_gen" (BType_Imm Bit1)``;
-
-fun bir_symb_analysis_init_gen pcond_symb_o birs_state_init_lbl bspec_pre_tm birenvtyl_def =
-  let
-    val bprog_envtyl_tm = (fst o dest_eq o concl) birenvtyl_def;
-
-    val bsysprecond_tm_f = Option.getOpt (Option.map (fn tm => fn x => ``BExp_BinExp BIExp_And (^x) (BExp_Den (^tm))``) pcond_symb_o, I);
-    val mk_bsysprecond_pcond_thm =
-      (computeLib.RESTR_EVAL_CONV [``birs_eval_exp``] THENC birs_stepLib.birs_eval_exp_CONV)
-        (bsysprecond_tm_f ``mk_bsysprecond ^bspec_pre_tm ^bprog_envtyl_tm``);
-    val birs_pcond_tm = (snd o dest_eq o concl) mk_bsysprecond_pcond_thm;
-
-    val senv_GEN_list_thm = (REWRITE_CONV [birenvtyl_def] THENC EVAL THENC REWRITE_CONV [GSYM birs_gen_env_thm, GSYM birs_gen_env_NULL_thm]) ``bir_senv_GEN_list ^bprog_envtyl_tm``;
-    val birs_env_tm = (snd o dest_eq o concl) senv_GEN_list_thm;
-
-    val pcond_is_sat = bir_smtLib.bir_smt_check_sat false birs_pcond_tm;
-    val _ = if pcond_is_sat then () else
-      raise ERR "bir_symb_analysis_init_gen" "initial pathcondition is not satisfiable; it seems to contain a contradiction";
-
-    val birs_state_init = ``<|
-      bsst_pc       := ^birs_state_init_lbl;
-      bsst_environ  := ^birs_env_tm;
-      bsst_status   := BST_Running;
-      bsst_pcond    := ^birs_pcond_tm
-    |>``;
-  in
-    (birs_state_init, senv_GEN_list_thm, mk_bsysprecond_pcond_thm)
-  end;
-
-fun bir_symb_analysis bprog_tm birs_end_lbls birs_state =
- let
-   val timer_symbanalysis = holba_miscLib.timer_start 0;
-   val timer_symbanalysis_last = ref (holba_miscLib.timer_start 0);
-
-   open birs_execLib;
-   val birs_rule_SUBST_thm = birs_rule_SUBST_prog_fun bprog_tm;
-   fun birs_post_step_fun (t, (last_pc, last_stmt)) = (
-      (fn t => (
-        holba_miscLib.timer_stop (fn delta_s => print ("running since " ^ delta_s ^ "\n")) timer_symbanalysis;
-        holba_miscLib.timer_stop (fn delta_s => print ("time since last step " ^ delta_s ^ "\n")) (!timer_symbanalysis_last);
-        timer_symbanalysis_last := holba_miscLib.timer_start 0;
-        (*print_term ((last o pairSyntax.strip_pair o snd o dest_comb o concl) t);*)
-        t)) o
-      apply_if_assign last_stmt (birs_rule_SUBST_trysimp_fun birs_rule_SUBST_thm (!birs_simp_select)) o
-      birs_rule_tryprune_fun birs_rulesTheory.branch_prune1_spec_thm o
-      birs_rule_tryprune_fun birs_rulesTheory.branch_prune2_spec_thm o
-      birs_rule_tryjustassert_fun true
-    ) t;
- in
-   birs_driveLib.bir_symb_exec_to (bprog_tm, birs_post_step_fun) birs_end_lbls birs_state
- end (* let *)
-
-
-fun bir_symb_analysis_thm_gen pcond_symb_o bir_prog_def
+fun bir_symb_analysis_thm bir_prog_def
  init_addr_def end_addr_defs
  bspec_pre_def birenvtyl_def =
  let
@@ -92,7 +24,7 @@ fun bir_symb_analysis_thm_gen pcond_symb_o bir_prog_def
 
    val bprog_tm = (fst o dest_eq o concl) bir_prog_def;
    val init_addr_tm = (snd o dest_eq o concl) init_addr_def;
-   val birs_state_init_lbl_tm =
+   val init_lbl =
     (snd o dest_eq o concl o EVAL) ``bir_block_pc (BL_Address ^(gen_mk_Imm init_addr_tm))``;
    val birs_state_end_tm_lbls =
     List.map 
@@ -102,18 +34,21 @@ fun bir_symb_analysis_thm_gen pcond_symb_o bir_prog_def
        end) end_addr_defs;
    val bspec_pre_tm = (lhs o snd o strip_forall o concl) bspec_pre_def;
 
-   val (birs_state_init, birs_env_thm, bsysprecond_thm) =
-     bir_symb_analysis_init_gen pcond_symb_o birs_state_init_lbl_tm bspec_pre_tm birenvtyl_def;
-   val symb_analysis_thm = bir_symb_analysis
-    bprog_tm birs_state_end_tm_lbls birs_state_init;
-   val symb_analysis_fix_thm = CONV_RULE (RAND_CONV (LAND_CONV (REWRITE_CONV [GSYM birs_env_thm]))) symb_analysis_thm;
+   val birs_state_init =
+     birs_driveLib.birs_analysis_init birenvtyl_def bspec_pre_tm init_lbl;
+
+   val symb_analysis_thm =
+     birs_driveLib.birs_exec_to
+       bprog_tm
+       (birs_strategiesLib.birs_post_step_riscv_default)
+       (fn _ => NONE)
+       (birs_strategiesLib.not_at_lbls birs_state_end_tm_lbls)
+       birs_state_init;
 
    val _ = holba_miscLib.timer_stop (fn delta_s => print ("\n======\n > bir_symb_analysis_thm took " ^ delta_s ^ "\n")) timer;
  in
-   (bsysprecond_thm, symb_analysis_fix_thm)
+   symb_analysis_thm
  end (* let *)
-
-val bir_symb_analysis_thm = bir_symb_analysis_thm_gen NONE;
 
 end (* local *)
 
@@ -152,8 +87,15 @@ fun bir_symb_transfer
  bspec_pre_tm bspec_post_tm
  bir_prog_def birenvtyl_def
  bspec_pre_def bspec_post_def prog_vars_list_def
- symb_analysis_thm bsysprecond_thm prog_vars_thm =
- let 
+ symb_analysis_thm prog_vars_thm =
+ let
+   val (bsysprecond_thm, symb_analysis_thm) =
+     birs_transferLib.prepare_transfer
+       birenvtyl_def
+       ``BExp_Const (Imm1 1w)``
+       ((lhs o snd o strip_forall o concl) bspec_pre_def)
+       symb_analysis_thm;
+
    val birs_state_ss = rewrites (type_rws ``:birs_state_t``);
    val bprog_tm = (fst o dest_eq o concl) bir_prog_def;
    val prog_vars_list_tm = (fst o dest_eq o concl) prog_vars_list_def;
@@ -368,7 +310,7 @@ fun bir_symb_transfer_thm
  bir_prog_def init_addr_def end_addr_def
  bspec_pre_def bspec_post_def
  birenvtyl_def prog_vars_list_def
- symb_analysis_thm bsysprecond_thm prog_vars_thm =
+ symb_analysis_thm prog_vars_thm =
  let
    val init_addr_tm = (snd o dest_eq o concl) init_addr_def;
    val end_addr_tm = (snd o dest_eq o concl) end_addr_def;
@@ -380,7 +322,7 @@ fun bir_symb_transfer_thm
      bspec_pre_tm bspec_post_tm
      bir_prog_def birenvtyl_def
      bspec_pre_def bspec_post_def prog_vars_list_def
-     symb_analysis_thm bsysprecond_thm prog_vars_thm
+     symb_analysis_thm prog_vars_thm
  end (* let *)
 
 end (* local *)
@@ -420,8 +362,15 @@ fun bir_symb_transfer_two
  bspec_pre_tm bspec_post_1_tm bspec_post_2_tm
  bir_prog_def birenvtyl_def
  bspec_pre_def bspec_post_1_def bspec_post_2_def prog_vars_list_def
- symb_analysis_thm bsysprecond_thm prog_vars_thm =
+ symb_analysis_thm prog_vars_thm =
  let
+   val (bsysprecond_thm, symb_analysis_thm) =
+     birs_transferLib.prepare_transfer
+       birenvtyl_def
+       ``BExp_Const (Imm1 1w)``
+       ((lhs o snd o strip_forall o concl) bspec_pre_def)
+       symb_analysis_thm;
+
    val birs_state_ss = rewrites (type_rws ``:birs_state_t``);
    val bprog_tm = (fst o dest_eq o concl) bir_prog_def;
    val prog_vars_list_tm = (fst o dest_eq o concl) prog_vars_list_def;
@@ -688,7 +637,7 @@ fun bir_symb_transfer_two_thm
   init_addr_def end_addr_1_def end_addr_2_def  
   bspec_pre_def bspec_post_1_def bspec_post_2_def
   birenvtyl_def prog_vars_list_def
-  symb_analysis_thm bsysprecond_thm prog_vars_thm =
+  symb_analysis_thm prog_vars_thm =
   let
     val init_addr_tm = (snd o dest_eq o concl) init_addr_def;
     val end_addr_1_tm = (snd o dest_eq o concl) end_addr_1_def;
@@ -702,7 +651,7 @@ fun bir_symb_transfer_two_thm
      bspec_pre_tm bspec_post_1_tm bspec_post_2_tm
      bir_prog_def birenvtyl_def
      bspec_pre_def bspec_post_1_def bspec_post_2_def prog_vars_list_def
-     symb_analysis_thm bsysprecond_thm prog_vars_thm
+     symb_analysis_thm prog_vars_thm
   end (* let *)
 
 end (* local *)
